SciLean/Tactic/DataSynth/HasRevFDeriv.lean
@@ -2,6 +2,7 @@ import SciLean.Analysis.Calculus.RevFDeriv
 import SciLean.Tactic.DataSynth.Attr
 import SciLean.Tactic.DataSynth.Elab
 import SciLean.Tactic.LSimp.Elab
+import SciLean.Tactic.Autodiff
 
 namespace SciLean
 
@@ -9,6 +10,39 @@ variable {R : Type} [RCLike R]
   {X : Type} [NormedAddCommGroup X] [AdjointSpace R X] [CompleteSpace X]
   {Y : Type} [NormedAddCommGroup Y] [AdjointSpace R Y] [CompleteSpace Y]
   {Z : Type} [NormedAddCommGroup Z] [AdjointSpace R Z] [CompleteSpace Z]
+  {X₁ : Type} [NormedAddCommGroup X₁] [AdjointSpace R X₁] [CompleteSpace X₁]
+  {X₂ : Type} [NormedAddCommGroup X₂] [AdjointSpace R X₂] [CompleteSpace X₂]
+
+syntax "let'" "(" ident,* ")" ":=" term ";" term : term
+
+macro_rules
+| `(let' ($x,$y) := $v; $b) =>
+  `(let x := $v
+    let $x := Prod.fst x
+    let $y := Prod.snd x
+    $b)
+| `(let' ($x,$y,$z) := $v; $b) =>
+  `(let x := $v
+    let $x := Prod.fst x
+    let $y := Prod.fst (Prod.snd x)
+    let $z := Prod.snd (Prod.snd x)
+    $b)
+
+| `(let' ($x,$y,$z,$w) := $v; $b) =>
+  `(let x := $v
+    let $x := Prod.fst x
+    let $y := Prod.fst (Prod.snd x)
+    let $z := Prod.fst (Prod.snd (Prod.snd x))
+    let $w := Prod.snd (Prod.snd (Prod.snd x))
+    $b)
+
+macro "let'" "(" "(" x:ident "," y:ident ")" "," z:ident ")" ":=" v:term ";" b:term : term =>
+  `(let x := $v
+    let $x := x.1.1
+    let $y := x.1.2
+    let $z := x.2
+    $b)
+
 
 variable (R)
 @[data_synth out f' in f]
@@ -32,6 +66,24 @@ theorem const_rule (y : Y) :  HasRevFDeriv R (fun x : X => y) (fun x => (y, fun 
   constructor
   · fun_trans
   · fun_prop
+
+
+omit [CompleteSpace X] [CompleteSpace Y] [CompleteSpace X₁] [AdjointSpace R X₂] [CompleteSpace X₂] in
+theorem proj_rule (f : X → Y) {g'}
+    (g : X₁ → Y) (p₁ : X → X₁) (p₂ : X → X₂) (q : X₁ → X₂ → X)
+    (hg : HasRevFDeriv R g g') :
+    HasRevFDeriv R f (fun x =>
+      let x₁ := p₁ x
+      let' (y,dg) := g' x₁;
+      (y, fun dy =>
+        let dz := dg dy
+        q dz 0)) := by sorry_proof
+
+
+#check LinearIsometry
+
+
+
 
 theorem comp_rule (f : Y → Z) (g : X → Y) (f' g')
     (hf : HasRevFDeriv R f f') (hg : HasRevFDeriv R g g') :
@@ -129,6 +181,27 @@ theorem Prod.snd.arg_self.HasRevFDeriv_rule
   · intro dx; fun_trans only; simp_all
   · fun_prop
 
+@[data_synth]
+theorem Prod.fst.arg_self.HasRevFDeriv_rule' :
+  HasRevFDeriv R
+    (fun x : X×Y => x.1)
+    (fun x =>
+      (x.1, fun dz => (dz,0))) := by
+  constructor
+  · intro dx; fun_trans only
+  · fun_prop
+
+
+@[data_synth]
+theorem Prod.snd.arg_self.HasRevFDeriv_rule' :
+  HasRevFDeriv R
+    (fun x : X×Y => x.2)
+    (fun x =>
+      (x.2, fun dz => (0,dz))) := by
+  constructor
+  · intro dx; fun_trans only
+  · fun_prop
+
 
 @[data_synth]
 theorem HAdd.hAdd.arg_a0a1.HasRevFDeriv_rule
@@ -189,6 +262,18 @@ theorem HMul.hMul.arg_a0a1.HasRevFDeriv_rule
   · intro dx; fun_trans only; simp_all
   · fun_prop
 
+open ComplexConjugate
+@[data_synth]
+theorem HMul.hMul.arg_a0a1.HasRevFDeriv_rule' :
+    HasRevFDeriv R (fun x : R×R => x.1 * x.2)
+      (fun x =>
+        (x.1 * x.2, fun dx =>
+           ((conj x.2) * dx, (conj x.1) * dx))) := by
+  constructor
+  · intro dx; fun_trans only; simp_all
+  · fun_prop
+
+
 
 omit [CompleteSpace X] [CompleteSpace Y] in
 theorem HasRevFDeriv.revFDeriv {f : X → Y} {f'} (hf : HasRevFDeriv R f f') :
@@ -199,66 +284,55 @@ theorem HasRevFDeriv.revFDeriv {f : X → Y} {f'} (hf : HasRevFDeriv R f f') :
 
 
 
-open SciLean Lean Meta in
-simproc [] dataSynthRevFDeriv (revFDeriv _ _ _) := fun e => do
+-- open SciLean Lean Meta in
+-- simproc [] dataSynthRevFDeriv (revFDeriv _ _ _) := fun e => do
 
-  let .mkApp2 _ f x := e | return .continue
-  let R := e.getArg! 0
+--   let .mkApp2 _ f x := e | return .continue
+--   let R := e.getArg! 0
 
-  let h ← mkAppM ``HasRevFDeriv #[R,f]
-  let (xs,_) ← forallMetaTelescope (← inferType h)
-  let h := h.beta #[xs[0]!, x]
+--   let h ← mkAppM ``HasRevFDeriv #[R,f]
+--   let (xs,_) ← forallMetaTelescope (← inferType h)
+--   let h := h.beta #[xs[0]!, x]
 
-  let some goal ← Tactic.DataSynth.isDataSynthGoal? h
-    | return .continue
+--   let some goal ← Tactic.DataSynth.isDataSynthGoal? h
+--     | return .continue
 
-  let (some r,_) ← Tactic.DataSynth.dataSynth goal |>.run {} |>.run {}
-    | return .continue
+--   let (some r,_) ← Tactic.DataSynth.dataSynth goal |>.run {} |>.run {}
+--     | return .continue
 
-  let e' := r.xs[0]!.beta #[x]
+--   let e' := r.xs[0]!.beta #[x]
 
-  return .visit { expr := e', proof? := ← mkAppM ``HasRevFDeriv.revFDeriv #[r.proof] }
-
-
-set_option trace.Meta.Tactic.data_synth true in
-set_option trace.Meta.Tactic.data_synth.input true in
-
-example : (revFDeriv R (fun x : R => x * x * x) 2)
-          =
-          fun dx => (2 * 2 * 2, 2 * 2 * dx + (2 * dx + dx * 2) * 2) := by
-  conv =>
-    lhs
-    simp -zeta [dataSynthRevFDeriv]
+--   return .visit { expr := e', proof? := ← mkAppM ``HasRevFDeriv.revFDeriv #[r.proof] }
 
 
 
-set_option trace.Meta.Tactic.data_synth true in
-set_option trace.Meta.Tactic.data_synth.input true in
-example : (revFDeriv R (fun x : R => let y := x * x; y * x) 2)
-          =
-          fun dx => (2 * 2 * 2, 2 * 2 * dx + (2 * dx + dx * 2) * 2) := by
-  conv =>
-    lhs
-    simp -zeta [dataSynthRevFDeriv]
-
-
-
-set_option trace.Meta.Tactic.data_synth true in
-#check (HasRevFDeriv R (fun x : R => x) _ )
+#check (HasRevFDeriv R (fun x : R => let y := x; x) _ )
   rewrite_by
-    data_synth
+    data_synth -normalizeLet +normalizeCore
 
+#exit
 
 #check (HasRevFDeriv R (fun x : R => x*x) _ )
   rewrite_by
     data_synth
 
+#check (HasRevFDeriv R (fun x : R => x*x*x*x*x) _ )
+  rewrite_by
+    data_synth
+
+
+#check (HasRevFDeriv R (fun x : R×R => x.1 * x.2) _) rewrite_by
+              data_synth
+
+#check (HasRevFDeriv R (fun x : R×R => x.2 * x.1) _) rewrite_by
+              data_synth
+
 
 set_option trace.Meta.Tactic.data_synth true in
 set_option trace.Meta.Tactic.data_synth.normalize true in
-#check (HasRevFDeriv R (fun x : R => let y := x; x) _ )
+#check (HasRevFDeriv R (fun x : R => let y := x; y+y) _ )
   rewrite_by
-    data_synth
+    data_synth -normalizeLet
 
 
 #check SciLean.HasRevFDeriv.let_rule
@@ -273,7 +347,105 @@ set_option trace.Meta.Tactic.data_synth.normalize true in
   rewrite_by
     data_synth
 
+set_option profiler true in
+set_option trace.Meta.Tactic.data_synth true in
+set_option trace.Meta.Tactic.data_synth.normalize true in
+set_option trace.Meta.Tactic.data_synth.input true in
+#check (HasRevFDeriv R (fun x : R =>
+            let x₁ := x
+            x) _) rewrite_by
+              data_synth
 
+
+set_option profiler true in
+set_option trace.Meta.Tactic.data_synth true in
+set_option trace.Meta.Tactic.data_synth.normalize true in
+set_option trace.Meta.Tactic.data_synth.input true in
+#check (HasRevFDeriv R (fun x : R =>
+            let x₁ := x*x*x
+            x*x₁) _) rewrite_by
+              data_synth
+
+
+set_option profiler true in
+set_option trace.Meta.Tactic.data_synth true in
+set_option trace.Meta.Tactic.data_synth.normalize true in
+set_option trace.Meta.Tactic.data_synth.input true in
+#check (HasRevFDeriv R (fun x : R =>
+            let x₁ := x*x
+            let x₂ := x*x₁
+            let x₃ := x*x₂
+            let x₄ := x*x₃
+            x*x₄) _) rewrite_by
+              data_synth
+
+
+
+
+set_option profiler true in
+set_option trace.Meta.Tactic.data_synth true in
+set_option trace.Meta.Tactic.data_synth.normalize true in
+set_option trace.Meta.Tactic.data_synth.input true in
+#check (HasRevFDeriv R (fun x : R =>
+            let x₁ := x*x
+            let x₂ := x*x₁
+            let x₃ := x*x₁*x₂
+            x*x₁*x₂*x₃) _) rewrite_by
+              data_synth +normalizeLet'
+
+-- set_option profiler true in
+-- #check (revFDeriv R (fun x : R =>
+--             let x₁ := x*x
+--             let x₂ := x*x₁
+--             let x₃ := x*x₁*x₂
+--             x*x₁*x₂*x₃) rewrite_by autodiff
+
+
+
+set_option profiler true in
+set_option trace.Meta.Tactic.data_synth true in
+set_option trace.Meta.Tactic.data_synth.normalize true in
+set_option trace.Meta.Tactic.data_synth.input true in
+#check (HasRevFDeriv R (fun x : R =>
+            let x₁ := x*x
+            let x₂ := x*x₁
+            let x₃ := x*x₁*x₂
+            let x₄ := x*x₁*x₂*x₃
+            x*x₁*x₂*x₃*x₄) _) rewrite_by
+              data_synth
+
+#exit
+
+set_option profiler true in
+set_option trace.Meta.Tactic.data_synth true in
+set_option trace.Meta.Tactic.data_synth.normalize true in
+set_option trace.Meta.Tactic.data_synth.input true in
+#check (HasRevFDeriv R (fun x : R =>
+            let x₁ := x*x
+            let x₂ := x*x₁
+            let x₃ := x*x₁*x₂
+            let x₄ := x*x₁*x₂*x₃
+            let x₅ := x*x₁*x₂*x₃*x₄
+            x*x₁*x₂*x₃*x₄*x₅) _) rewrite_by
+              data_synth -normalizeLet +normalizeLet'
+
+
+#exit
+set_option pp.deepTerms.threshold 10000000
+#check (HasRevFDeriv R (fun x : R =>
+            let x₁ := x*x
+            let x₂ := x*x₁
+            let x₃ := x*x₁*x₂
+            let x₄ := x*x₁*x₂*x₃
+            x*x₁*x₂*x₃*x₄) _) rewrite_by
+              data_synth
+
+
+
+#check (HasRevFDeriv R (fun x : R =>
+            let x₁ := x*x
+            x*x₁) _) rewrite_by
+              data_synth
 
 
 set_option trace.Meta.Tactic.data_synth true in
