SciLean/Tactic/DataSynth/HasRevFDerivUpdate.lean
@@ -1,0 +1,381 @@
+import SciLean.Tactic.DataSynth.HasRevFDeriv
+
+set_option linter.unusedVariables false
+
+namespace SciLean
+
+variable {R : Type} [RCLike R]
+  {X : Type} [NormedAddCommGroup X] [AdjointSpace R X] [CompleteSpace X]
+  {Y : Type} [NormedAddCommGroup Y] [AdjointSpace R Y] [CompleteSpace Y]
+  {Z : Type} [NormedAddCommGroup Z] [AdjointSpace R Z] [CompleteSpace Z]
+  {X₁ : Type} [NormedAddCommGroup X₁] [AdjointSpace R X₁] [CompleteSpace X₁]
+  {X₂ : Type} [NormedAddCommGroup X₂] [AdjointSpace R X₂] [CompleteSpace X₂]
+
+
+variable (R)
+@[data_synth out f' in f]
+structure HasRevFDerivUpdate (f : X → Y) (f' : X → Y×(Y→X→X))  where
+  val : ∀ x, f' x
+             =
+             let' (y,df) := revFDeriv R f x;
+             (y, fun dy dx => dx + df dy)
+  prop : Differentiable R f
+variable {R}
+
+
+namespace HasRevFDerivUpdate
+
+@[data_synth]
+theorem id_rule : HasRevFDerivUpdate R (fun x : X => x) (fun x => (x, fun dx dx₀ => dx₀ + dx)) := by
+  constructor
+  · fun_trans
+  · fun_prop
+
+
+@[data_synth]
+theorem const_rule (y : Y) :  HasRevFDerivUpdate R (fun x : X => y) (fun x => (y, fun _ dx => dx)) := by
+  constructor
+  · fun_trans
+  · fun_prop
+
+
+theorem comp_rule (f : Y → Z) (g : X → Y) (f' g')
+    (hf : HasRevFDerivUpdate R f f') (hg : HasRevFDerivUpdate R g g') :
+    HasRevFDerivUpdate R
+      (fun x : X => f (g x))
+      (fun x =>
+        let' (y,dg) := g' x;
+        let' (z,df) := f' y;
+        (z, fun dz dx =>
+              let dy := df dz 0
+              dg dy dx)) := by
+
+  cases hf; cases hg
+  constructor
+  · intro dx; fun_trans only; simp_all
+  · fun_prop
+
+
+theorem let_rule (g : X → Y) (f : Y → X → Z) {f' g'}
+    (hg : HasRevFDerivUpdate R g g')
+    (hf : HasRevFDerivUpdate R (fun yx : Y×X => f yx.1 yx.2) f')  :
+    HasRevFDerivUpdate R
+      (fun x : X => let y := g x; f y x)
+      (fun x =>
+        let' (y,dg) := g' x;
+        let' (z,df) := f' (y,x);
+        (z, fun dz dx =>
+          let' (dy,dx) := df dz (0,dx);
+          dg dy dx)) := by
+
+  cases hf; cases hg
+  constructor
+  · intro dx; fun_trans only; simp_all; ac_rfl
+  · fun_prop
+
+
+omit [CompleteSpace X] [CompleteSpace Y] [CompleteSpace X₁] [AdjointSpace R X₂] [CompleteSpace X₂] [NormedAddCommGroup X₂] in
+theorem proj_rule (f : X → Y) {g'}
+    (g : X₁ → Y) (p₁ : X → X₁) (p₂ : X → X₂) (q : X₁ → X₂ → X)
+    (hg : HasRevFDerivUpdate R g g') :
+    HasRevFDerivUpdate R f (fun x =>
+      let x₁ := p₁ x
+      let' (y,dg) := g' x₁;
+      (y, fun dy dx =>
+        let dx₁ := p₁ dx
+        let dx₂ := p₂ dx
+        let dx₁ := dg dy dx₁
+        q dx₁ dx₂)) := by sorry_proof
+
+
+end HasRevFDerivUpdate
+
+@[data_synth]
+theorem Prod.mk.arg_a0a1.HasRevFDerivUpdate_rule
+  (f : X → Y) (g : X → Z) (f' g')
+  (hf : HasRevFDerivUpdate R f f') (hg : HasRevFDerivUpdate R g g') :
+  HasRevFDerivUpdate R
+    (fun x => (f x, g x))
+    (fun x =>
+      let' (y,df) := f' x;
+      let' (z,dg) := g' x;
+      ((y,z), fun dyz dx =>
+        let' (dy,dz) := dyz;
+        let dx := df dy dx
+        dg dz dx)) := by
+
+  cases hf; cases hg
+  constructor
+  · intro dx; fun_trans only; simp_all; ac_rfl
+  · fun_prop
+
+@[data_synth]
+theorem Prod.fst.arg_self.HasRevFDerivUpdate_rule
+  (f : X → Y×Z) (f')
+  (hf : HasRevFDerivUpdate R f f') :
+  HasRevFDerivUpdate R
+    (fun x => (f x).1)
+    (fun x =>
+      let' ((y,z),df) := f' x;
+      (y, fun dy dx => df (dy,0) dx)) := by
+  cases hf
+  constructor
+  · intro dx; fun_trans only; simp_all
+  · fun_prop
+
+@[data_synth]
+theorem Prod.snd.arg_self.HasRevFDerivUpdate_rule
+  (f : X → Y×Z) (f')
+  (hf : HasRevFDerivUpdate R f f') :
+  HasRevFDerivUpdate R
+    (fun x => (f x).2)
+    (fun x =>
+      let' ((y,z),df) := f' x;
+      (z, fun dz dx => df (0,dz) dx)) := by
+  cases hf
+  constructor
+  · intro dx; fun_trans only; simp_all
+  · fun_prop
+
+
+@[data_synth]
+theorem HAdd.hAdd.arg_a0a1.HasRevFDerivUpdate_rule
+    (f g : X → Y) (f' g')
+    (hf : HasRevFDerivUpdate R f f') (hg : HasRevFDerivUpdate R g g') :
+    HasRevFDerivUpdate R (fun x => f x + g x)
+      (fun x =>
+        let' (y,df) := f' x;
+        let' (z,dg) := g' x;
+        (y + z, fun dy dx =>
+                  let dx := df dy dx
+                  dg dy dx)) := by
+  cases hf; cases hg
+  constructor
+  · intro dx; fun_trans only; simp_all; ac_rfl
+  · fun_prop
+
+
+@[data_synth]
+theorem HSub.hSub.arg_a0a1.HasRevFDerivUpdate_rule
+    (f g : X → Y) (f' g')
+    (hf : HasRevFDerivUpdate R f f') (hg : HasRevFDerivUpdate R g g') :
+    HasRevFDerivUpdate R (fun x => f x - g x)
+      (fun x =>
+        let' (y,df) := f' x;
+        let' (z,dg) := g' x;
+        (y - z, fun dy dx =>
+                  let dx := df dy dx
+                  dg (-dy) dx)) := by
+  cases hf; cases hg
+  constructor
+  · intro dx; fun_trans only;
+    simp_all[revFDeriv,neg_pull]
+    funext dy dx
+    abel
+  · fun_prop
+
+
+open ComplexConjugate
+@[data_synth]
+theorem HMul.hMul.arg_a0a1.HasRevFDerivUpdate_rule
+    (f g : X → R) (f' g')
+    (hf : HasRevFDerivUpdate R f f') (hg : HasRevFDerivUpdate R g g') :
+    HasRevFDerivUpdate R (fun x => f x * g x)
+      (fun x =>
+        let' (y,df) := f' x;
+        let' (z,dg) := g' x;
+        (y * z, fun dy dx =>
+           let dy₁ := (conj z) • dy
+           let dy₂ := (conj y) • dy
+           let dx := df dy₁ dx
+           let dx := dg dy₂ dx
+           dx)) := by
+  cases hf; cases hg
+  constructor
+  · intro dx; fun_trans only; simp_all
+    funext dy dx
+    simp[revFDeriv,smul_push]
+    ac_rfl
+  · fun_prop
+
+
+set_option trace.Meta.Tactic.data_synth true in
+#check (HasRevFDerivUpdate R (fun x : R => x*x*x*x*x) _ )
+  rewrite_by
+    data_synth
+
+
+#check (HasRevFDerivUpdate R (fun x : R×R => x.1 * x.2 * x.1 * x.1 * x.2) _) rewrite_by
+              data_synth
+
+
+#check (HasRevFDerivUpdate R (fun x : R×R => x.2 * x.1) _) rewrite_by
+              data_synth
+
+
+set_option trace.Meta.Tactic.data_synth true in
+#check (HasRevFDerivUpdate R (fun x : R×R×R => x.1 * x.2.1) _) rewrite_by
+  data_synth
+
+
+set_option trace.Meta.Tactic.data_synth true in
+set_option trace.Meta.Tactic.data_synth.normalize true in
+#check (HasRevFDerivUpdate R (fun x : R => let y := x; y+y) _ )
+  rewrite_by
+    data_synth
+
+
+#check SciLean.HasRevFDerivUpdate.let_rule
+
+
+#check (HasRevFDerivUpdate R (fun x : R => x*x*x*x*x*x*x*x*x*x*x*x*x*x*x*x*x*x*x*x*x) _ )
+  rewrite_by
+    data_synth
+
+#check (HasRevFDerivUpdate R (fun x : R×R×R×R => x.1) _) rewrite_by
+              data_synth
+
+set_option pp.deepTerms.threshold 1000000000000000
+
+
+set_option profiler true in
+set_option trace.Meta.Tactic.data_synth true in
+set_option trace.Meta.Tactic.data_synth.normalize true in
+set_option trace.Meta.Tactic.data_synth.input true in
+#check (HasRevFDerivUpdate R (fun x : R =>
+            let y := x * x
+            let z := y * y
+            z) _) rewrite_by
+              data_synth
+
+
+        -- (fun yx =>
+        --   let z := yx.1 * yx.1;
+        --   z)
+
+
+set_option profiler true in
+set_option trace.Meta.Tactic.data_synth true in
+set_option trace.Meta.Tactic.data_synth.normalize true in
+set_option trace.Meta.Tactic.data_synth.input true in
+#check (HasRevFDerivUpdate R (fun x : R =>
+            let x₁ := x*x*x
+            x*x₁) _) rewrite_by
+              data_synth
+
+
+set_option profiler true in
+set_option trace.Meta.Tactic.data_synth true in
+set_option trace.Meta.Tactic.data_synth.normalize true in
+set_option trace.Meta.Tactic.data_synth.input true in
+#check (HasRevFDerivUpdate R (fun x : R =>
+            let x₁ := x*x
+            let x₂ := x*x₁
+            let x₃ := x*x₂
+            let x₄ := x*x₃
+            x*x₄) _) rewrite_by
+              data_synth
+
+
+
+set_option profiler true in
+set_option trace.Meta.Tactic.data_synth true in
+set_option trace.Meta.Tactic.data_synth.normalize true in
+set_option trace.Meta.Tactic.data_synth.input true in
+#check (HasRevFDerivUpdate R (fun x : R =>
+            let x₁ := x*x
+            let x₂ := x*x₁
+            let x₃ := x*x₁*x₂
+            x*x₁*x₂*x₃) _) rewrite_by
+              data_synth
+
+
+set_option trace.Meta.Tactic.data_synth true in
+set_option trace.Meta.Tactic.data_synth.normalize true in
+set_option trace.Meta.Tactic.data_synth.input true in
+#check (HasRevFDerivUpdate R (fun x : R =>
+            let x₁ := x
+            let x₂ := x*x₁
+            x*x₁*x₂) _) rewrite_by
+              data_synth
+
+-- set_option profiler true in
+-- #check (revFDeriv R (fun x : R =>
+--             let x₁ := x*x
+--             let x₂ := x*x₁
+--             let x₃ := x*x₁*x₂
+--             x*x₁*x₂*x₃) rewrite_by autodiff
+set_option trace.Meta.Tactic.data_synth true in
+set_option trace.Meta.Tactic.data_synth.input true in
+#check (HasRevFDerivUpdate R (fun x : R => let y := (x,x); y) _)
+   rewrite_by
+     data_synth
+
+
+set_option profiler true in
+set_option trace.Meta.Tactic.data_synth true in
+set_option trace.Meta.Tactic.data_synth.normalize true in
+set_option trace.Meta.Tactic.data_synth.input true in
+#check (HasRevFDerivUpdate R (fun x : R =>
+            let x₁ := x*x
+            let x₂ := x*x₁
+            let x₃ := x*x₁*x₂
+            let x₄ := x*x₁*x₂*x₃
+            x*x₁*x₂*x₃*x₄) _) rewrite_by
+              data_synth
+
+
+set_option pp.deepTerms.threshold 100000000000000
+set_option profiler true in
+-- set_option trace.Meta.Tactic.data_synth true in
+-- set_option trace.Meta.Tactic.data_synth.normalize true in
+-- set_option trace.Meta.Tactic.data_synth.input true in
+#check (HasRevFDerivUpdate R (fun x : R =>
+            let x₁ := x*x
+            let x₂ := x*x₁
+            let x₃ := x*x₁*x₂
+            let x₄ := x*x₁*x₂*x₃
+            let x₅ := x*x₁*x₂*x₃*x₄
+            let x₆ := x*x₁*x₂*x₃*x₄*x₅
+            let x₇ := x*x₁*x₂*x₃*x₄*x₅*x₆
+            x*x₁*x₂*x₃*x₄*x₅*x₆*x₇) _) rewrite_by
+              data_synth -normalizeLet +normalizeCore
+
+
+
+#exit
+set_option pp.deepTerms.threshold 10000000
+#check (HasRevFDerivUpdate R (fun x : R =>
+            let x₁ := x*x
+            let x₂ := x*x₁
+            let x₃ := x*x₁*x₂
+            let x₄ := x*x₁*x₂*x₃
+            x*x₁*x₂*x₃*x₄) _) rewrite_by
+              data_synth
+
+
+
+#check (HasRevFDerivUpdate R (fun x : R =>
+            let x₁ := x*x
+            x*x₁) _) rewrite_by
+              data_synth
+
+
+set_option trace.Meta.Tactic.data_synth true in
+#check (HasRevFDerivUpdate R (fun x : R => let y := x * x; y * x) _ )
+  rewrite_by
+    data_synth
+
+
+
+set_option trace.Meta.Tactic.simp.rewrite true in
+#check (revFDeriv R (fun x : R => let x₁ := x * x; let x₂ := x*x₁; let x₃ := x*x₁*x₂; x*x₁*x₂*x₃) 2)
+  rewrite_by
+    simp -zeta only [dataSynthRevFDeriv]
+
+
+set_option profiler true in
+
+#check (HasRevFDerivUpdate R (fun x : R×R =>) _ 2)
+  rewrite_by
+    data_synth +lsimp -zeta
